in progress sparse merkle

Veritas.SparseMerkleVerifier.fst
@@ -11,15 +11,15 @@ open Veritas.Merkle
 //Allow the solver to invert inductive definitions at most once (ifuel)
 #push-options "--max_fuel 1 --max_ifuel 1 --initial_fuel 1 --initial_ifuel 1"
 
-(* 
- * The verifier consumes a log that consists of memory operations and 
+(*
+ * The verifier consumes a log that consists of memory operations and
  * additional "proof" objects and returns success of failure; we prove
- * that if the verifier returns success, then the underlying memory 
- * operations are read-write consistent 
+ * that if the verifier returns success, then the underlying memory
+ * operations are read-write consistent
  *)
 
 (* Each entry of the verifier log *)
-type verifier_log_entry = 
+type verifier_log_entry =
   | MemoryOp: o:memory_op -> verifier_log_entry
   | Add: a:merkle_addr -> v:sp_merkle_payload -> a':merkle_addr -> verifier_log_entry
   | Evict: a:merkle_addr -> a':merkle_addr -> verifier_log_entry
@@ -34,26 +34,26 @@ let is_evict (l:verifier_log) (i:vl_index l): Tot bool =
   Evict? (index l i)
 
 (* evicted address for an evict operation *)
-let evict_addr (l:verifier_log) (i:vl_index l{is_evict l i}): Tot merkle_addr = 
+let evict_addr (l:verifier_log) (i:vl_index l{is_evict l i}): Tot merkle_addr =
   Evict?.a (index l i)
 
 (* ancestor recording the evicted nodes hashes *)
-let evict_ancestor (l:verifier_log) (i:vl_index l{is_evict l i}): Tot merkle_addr = 
+let evict_ancestor (l:verifier_log) (i:vl_index l{is_evict l i}): Tot merkle_addr =
   Evict?.a' (index l i)
 
 (* is the ith operation an add *)
-let is_add (l:verifier_log) (i:vl_index l) = 
+let is_add (l:verifier_log) (i:vl_index l) =
   Add? (index l i)
 
 (* added address for an add operation *)
-let add_addr (l:verifier_log) (i:vl_index l{is_add l i}): Tot merkle_addr = 
+let add_addr (l:verifier_log) (i:vl_index l{is_add l i}): Tot merkle_addr =
   Add?.a (index l i)
 
 (* added payload for an add operation *)
 let add_payload (l:verifier_log) (i:vl_index l {is_add l i}): Tot sp_merkle_payload =
   Add?.v (index l i)
 
-let add_ancestor (l:verifier_log) (i:vl_index l {is_add l i}): Tot merkle_addr = 
+let add_ancestor (l:verifier_log) (i:vl_index l {is_add l i}): Tot merkle_addr =
   Add?.a' (index l i)
 
 (* is the ith operation a memory operation? *)
@@ -63,87 +63,95 @@ let is_memory_op (l:verifier_log) (i:vl_index l): Tot bool = MemoryOp? (index l 
 let memory_op_at (l:verifier_log) (i:vl_index l{is_memory_op l i}) = MemoryOp?.o (index l i)
 
 (* is the i'th operation a write operation *)
-let is_write_op (l:verifier_log) (i:vl_index l): Tot bool = 
+let is_write_op (l:verifier_log) (i:vl_index l): Tot bool =
   is_memory_op l i && Write? (memory_op_at l i)
 
 (* written value for a write operation *)
-let written_value (l:verifier_log) (i:vl_index l{is_write_op l i}): Tot payload = 
+let written_value (l:verifier_log) (i:vl_index l{is_write_op l i}): Tot payload =
   Write?.v (memory_op_at l i)
 
 (* is the ith operation a read operation *)
-let is_read_op (l:verifier_log) (i:vl_index l): Tot bool = 
+let is_read_op (l:verifier_log) (i:vl_index l): Tot bool =
   is_memory_op l i && Read? (memory_op_at l i)
 
 (* read value for a read operation *)
-let read_value (l:verifier_log) (i:vl_index l{is_read_op l i}): Tot payload = 
+let read_value (l:verifier_log) (i:vl_index l{is_read_op l i}): Tot payload =
   Read?.v (memory_op_at l i)
 
 (* Verifier cache of a subset of merkle_addr, merkle_payloads *)
 type verifier_cache = (a:merkle_addr) -> option (sp_merkle_payload_of_addr a)
 
 (* Does the cache contain a merkle addr? *)
-let cache_contains (vc:verifier_cache) (a:merkle_addr): Tot bool = 
+let cache_contains (vc:verifier_cache) (a:merkle_addr): Tot bool =
   Some? (vc a)
 
 (* Lookup the payload of an address in cache *)
 let cached_payload (cache:verifier_cache) (a:merkle_addr{cache_contains cache a}): Tot (sp_merkle_payload_of_addr a) =
   Some?.v (cache a)
 
-(* 
- * Update the cache. This is a pure update function that requires 
+(*
+ * Update the cache. This is a pure update function that requires
  * that cache contain an entry for the merkle address as a precondition
  *)
-let cache_update (cache:verifier_cache) 
-                 (a:merkle_addr{cache_contains cache a}) 
-                 (v:sp_merkle_payload_of_addr a): 
-  Tot (cache':verifier_cache{cache_contains cache' a}) = 
+let cache_update (cache:verifier_cache)
+                 (a:merkle_addr{cache_contains cache a})
+                 (v:sp_merkle_payload_of_addr a):
+  Tot (cache':verifier_cache{cache_contains cache' a}) =
   fun a' -> if a' = a then Some v else cache a'
 
-(* 
- * Update the cache to reflect a memory write, which translates to updating 
- * the leaf merkle node in the cache. This is a pure update function and we 
+(*
+ * Update the cache to reflect a memory write, which translates to updating
+ * the leaf merkle node in the cache. This is a pure update function and we
  * require the cache to contain an entry for the merkle addr as a precondition
  *)
 let cache_apply (cache:verifier_cache)
-                (o:memory_op{Write? o && 
+                (o:memory_op{Write? o &&
                              cache_contains cache (addr_to_merkle_leaf (address_of o))})
   : Tot (vc':verifier_cache{cache_contains vc' (addr_to_merkle_leaf (address_of o))}) =
   match o with
   | Read _ _ -> cache
   | Write a v -> cache_update cache (addr_to_merkle_leaf a) (SMkLeaf v)
-  
+
 (* Add a merkle_addr, payload to cache *)
 let cache_add (cache:verifier_cache)
-              (a:merkle_addr {not (cache_contains cache a)}) 
-              (v:sp_merkle_payload_of_addr a) 
+              (a:merkle_addr {not (cache_contains cache a)})
+              (v:sp_merkle_payload_of_addr a)
   : Tot (cache':verifier_cache {cache_contains cache' a}) =
   fun a' -> if a' = a then Some v else cache a'
 
 (* Evict a merkle_addr from cache *)
-let cache_evict (cache:verifier_cache) 
-                (a:merkle_addr{cache_contains cache a}) 
-  : Tot verifier_cache = 
+let cache_evict (cache:verifier_cache)
+                (a:merkle_addr{cache_contains cache a})
+  : Tot verifier_cache =
   fun a' -> if a' = a then None else cache a'
 
 (* Verifier state is the cache if valid *)
-noeq type verifier_state = 
-  | Failed: verifier_state 
+noeq type verifier_state =
+  | Failed: verifier_state
   | Valid: vc:verifier_cache -> verifier_state
 
-let is_hash_at_ancestor_correct (cache:verifier_cache)
-                                (a:merkle_non_root_addr)
-                                (v:sp_merkle_payload_of_addr a)
-                                (a': merkle_addr): Tot bool = 
-  (* check a' is an ancestor of a *)
-  if not (is_desc a a') then false
-  (* check a' is in the cache *)
-  else if not (cache_contains cache a') then false  
+let get_desc_hash (a: merkle_non_root_addr)
+                  (a':merkle_addr {is_proper_desc a a'})
+                  (v': sp_merkle_payload_of_addr a'):
+  Tot (dh:desc_hash) =
+  if is_desc a (LeftChild a') then
+    SMkInternal?.left v'
   else
-    let v' = cached_payload cache a' in
-    
-    admit()
+    SMkInternal?.right v'
 
-let verifier_step (e:verifier_log_entry) (vs:verifier_state): Tot verifier_state = 
+let update_desc_hash (a:merkle_addr) (v:sp_merkle_payload_of_addr a)
+                     (d:merkle_addr {is_proper_desc d a}) (h:hash_value): Tot (sp_merkle_payload_of_addr a) =
+  if is_desc d (LeftChild a) then
+    SMkInternal (Desc d h) (SMkInternal?.right v)
+  else
+    SMkInternal (SMkInternal?.left v) (Desc d h)
+
+let is_empty_or_null (a:merkle_addr) (v:sp_merkle_payload_of_addr a): Tot bool =
+  if is_merkle_leaf a then Null? (SMkLeaf?.value v)
+  else Empty? (SMkInternal?.left v) &&
+       Empty? (SMkInternal?. right v)
+
+let verifier_step (e:verifier_log_entry) (vs:verifier_state): Tot verifier_state =
   (* propagate failures *)
   if (Failed? vs) then Failed
   else
@@ -158,18 +166,306 @@ let verifier_step (e:verifier_log_entry) (vs:verifier_state): Tot verifier_state
           let payload = Some?.v optPayload in
           match o with
           (* For reads, the value read should correspond to the value in the cache *)
-          | Read _ v -> if v = SMkLeaf?.value payload then vs else Failed            
+          | Read _ v -> if v = SMkLeaf?.value payload then vs else Failed
           (* For writes, update the cache to reflect the write *)
           | Write a v -> Valid (cache_apply cache o))
-     | Add a v a' -> 
+     | Add a v a' ->
          (* Check cache contains merkle addr a *)
-         if cache_contains cache a then Failed 
+         if cache_contains cache a then Failed
          (* Root is never added *)
          else if is_merkle_root a then Failed
          (* Check the payload type corresponds to leaf/internal ness of address a *)
-         else if not (is_sp_payload_of_addr a v) then Failed 
-         (* check the hash of a v is stored at ancestor a' *)
-         else if not (is_hash_at_ancestor_correct cache a v a') then Failed 
-         (* All checks passed - add (a,v) to the cache *)
-         else Valid (cache_add cache a v)
-     | Evict a a' -> admit()
+         else if not (is_sp_payload_of_addr a v) then Failed
+         (* Check ancestor a' is in cache *)
+         else if not (cache_contains cache a') then Failed
+         (* check that a is a proper descendant of a' *)
+         else if not (is_proper_desc a a') then Failed
+
+         else (
+           let v' = cached_payload cache a' in
+           let dh' = get_desc_hash a a' v' in
+           let h = hashfn_sp v in
+           (* ancestor a' stores the address a and its hash *)
+           if not (Empty? dh') && a = Desc?.a dh' then
+             (* check the hash and add a to cache if hash check passes *)
+             if h = Desc?.h dh' then Valid (cache_add cache a v)
+             else Failed
+           (* if ancestor a' does not point to a, then a has to be empty *)
+           else if not (is_empty_or_null a v) then Failed
+
+           (* entire subtree l|r(a) subtree of a' empty *)
+           else if Empty? dh' then
+             (* if it is update a' to point to a *)
+             let v'_upd = update_desc_hash a' v' a h in
+             Valid (cache_add (cache_update cache a' v'_upd) a v)
+
+           (* if a' points to some other addr, that addr has to be a desc of a *)
+           else if not (is_proper_desc (Desc?.a dh') a) then Failed
+
+           else
+             let v_upd = update_desc_hash a v (Desc?.a dh') (Desc?.h dh') in
+             let v'_upd = update_desc_hash a' v' a (hashfn_sp v_upd) in
+             Valid (cache_add (cache_update cache a' v'_upd) a v_upd)
+         )
+     | Evict a a' ->
+         if not (cache_contains cache a && cache_contains cache a') then Failed
+         else if is_merkle_root a then Failed
+         else if not (is_proper_desc a a') then Failed
+         else
+           let v' = cached_payload cache a' in
+           let v = cached_payload cache a in
+           let h = hashfn_sp v in
+           let dh' = get_desc_hash a a' v' in
+           let v'_upd = update_desc_hash a' v' a h in
+           if not (Empty? dh') && a = Desc?.a dh' then
+             Valid (cache_evict (cache_update cache a' v'_upd) a)
+           else Failed
+
+(* Verifier for a given log, from a specified initial state *)
+let rec verifier_aux (l:verifier_log) (init_vs:verifier_state): Tot verifier_state
+  (decreases (length l)) =
+  let n = length l in
+  (* empty log *)
+  if n = 0 then init_vs
+  else
+    let l' = prefix l (n - 1) in
+    (* recurse *)
+    let vs' = verifier_aux l' init_vs in
+    let e' = index l (n - 1) in
+    verifier_step e' vs'
+
+(*
+ * Initial payload for every merkle node for init memory where each address
+ * contains Null
+ *)
+let init_payload (a:merkle_addr): Tot (sp_merkle_payload_of_addr a) =
+    if is_merkle_leaf a then
+      SMkLeaf Null
+    else
+      SMkInternal Empty Empty
+
+(* Initial cache contains only the merkle root *)
+let init_cache:verifier_cache =
+  fun a -> if is_merkle_root a then
+           Some (init_payload a)
+         else None
+
+(* Verifier for a log from the initial state *)
+let verifier (l:verifier_log): Tot verifier_state =
+  verifier_aux l (Valid init_cache)
+
+(* Does the verifier return Valid (success) for this log *)
+let verifiable (l:verifier_log): Tot bool =
+  Valid? (verifier l)
+
+(* Refinement type of logs that are verifiable *)
+type verifiable_log = l:verifier_log{verifiable l}
+
+(* If a log is verifiable, then each prefix of the log is also verifiable *)
+let rec lemma_verifiable_implies_prefix_verifiable (l:verifiable_log) (i:nat{i <= length l}):
+  Lemma (requires (True))
+        (ensures (verifiable (prefix l i)))
+        (decreases (length l))
+        [SMTPat (prefix l i)]
+        =
+  let n = length l in
+  if n = 0 then ()
+  else if i = n then ()
+  else
+    lemma_verifiable_implies_prefix_verifiable (prefix l (n - 1)) i
+
+
+(* is this log entry, an evict of a specified address *)
+let is_evict_of_addr (a:merkle_addr) (e:verifier_log_entry) =
+  Evict? e && Evict?.a e = a
+
+(* Does this log have some evict entry for address a *)
+let has_some_evict (l:verifier_log) (a:merkle_addr) = exists_sat_elems (is_evict_of_addr a) l
+
+(* Index of the last evict entry *)
+let last_evict_idx (l:verifier_log) (a:merkle_addr{has_some_evict l a}) =
+  last_index (is_evict_of_addr a) l
+
+(* Is this an add operation on address a *)
+let is_add_of_addr (a:merkle_addr) (e:verifier_log_entry) =
+  Add? e && Add?.a e = a
+
+(* Does thie log have some add entry for address a *)
+let has_some_add (l:verifier_log) (a:merkle_addr) = exists_sat_elems (is_add_of_addr a) l
+
+(* Index of the last add operation *)
+let last_add_idx (l:verifier_log) (a:merkle_addr{has_some_add l a}) =
+  last_index (is_add_of_addr a) l
+
+(* Is this log entry a write to address a *)
+let is_write_to_addr (a:merkle_leaf_addr) (e:verifier_log_entry) =
+  MemoryOp? e && is_write_to_addr (merkle_leaf_to_addr a) (MemoryOp?.o e)
+
+(* Does this log have some write to address a *)
+let has_some_write (l:verifiable_log) (a:merkle_leaf_addr) = exists_sat_elems (is_write_to_addr a) l
+
+(* Index of last write to address a *)
+let last_write_idx (l:verifiable_log) (a:merkle_leaf_addr{has_some_write l a}) =
+  last_index (is_write_to_addr a) l
+
+(* State of the cache after processing log l *)
+let cache_at_end (l:verifiable_log): Tot verifier_cache =
+  Valid?.vc (verifier l)
+
+(*
+ * We want to prove that if the verifier returns Valid for a log l, then the
+ * read-write operations in log l are rw-consistent unless there is a hash collision.
+ * To prove this, we develop a notion of evict-add consistency:
+ *
+ * A log is evict-add consistent, if every add sees the payload of the most recent evict
+ * to the same address or some initial value if there has been no previous evict
+ *
+ * We prove (1) evict-add consistency implies rw-consistency (2) a verifiable log that is
+ * not evict-add consistent implies a hash collision (that we construct)
+ *)
+
+(* payload of an evict operation *)
+let evict_payload (l:verifiable_log) (i:vl_index l{is_evict l i}):
+  Tot (sp_merkle_payload_of_addr (evict_addr l i)) =
+  let a = evict_addr l i in
+  let vs'' = verifier (prefix l i) in
+  lemma_prefix_index l (i + 1) i;
+  Some?.v ((Valid?.vc vs'') a)
+
+(*
+ * for a given address a, the last evict payload or init_payload if
+ * there exists no evicts for add
+ *)
+let last_evict_value_or_init (l:verifiable_log) (a:merkle_addr):
+  Tot (sp_merkle_payload_of_addr a) =
+  if has_some_evict l a then
+    evict_payload l (last_evict_idx l a)
+  else
+    init_payload a
+
+(* evict-add consistency (eac) for a verifiable log *)
+type evict_add_consistent (l:verifiable_log) = forall (i:vl_index l).
+    is_add l i  ==>
+    add_payload l i = last_evict_value_or_init (prefix l i) (add_addr l i)
+
+(* refinement of verifiable logs that are evict-add consistent *)
+type eac_log  = l:verifiable_log {evict_add_consistent l}
+
+(* Lemma: prefix of evict-add-consistent log is evict-add-consistent *)
+let lemma_eac_prefix (l:eac_log) (i:nat{i <= length l}):
+  Lemma (requires (True))
+        (ensures (evict_add_consistent (prefix l i)))
+        [SMTPat (prefix l i)]
+        =
+  let l' = prefix l i in
+  let aux (j:vl_index l'):
+    Lemma (requires is_add l' j)
+          (ensures add_payload l' j = last_evict_value_or_init (prefix l' j) (add_addr l' j))
+          [SMTPat(is_add l' j)] = ()
+  in
+  ()
+
+(* 
+ * return the first index i, such that prefix of l of length i is evict add consistent 
+ * and prefix of length (i + 1) is not
+ *)
+let rec search_first_non_eac_prefix (l:verifiable_log):
+  Tot (i:nat{i <= length l /\
+            evict_add_consistent (prefix l i) /\
+            (i < length l ==> (is_add l i &&
+                               add_payload l i <> last_evict_value_or_init (prefix l i)
+                                                                          (add_addr l i)))})
+  (decreases (length l)) =
+  let n = length l in
+  if n = 0 then 0
+  else
+    let l' = prefix l (n - 1) in
+    let i' = search_first_non_eac_prefix l' in
+    if i' < n - 1 then i'
+    else
+      if is_add l (n - 1) &&
+         add_payload l (n - 1) <> last_evict_value_or_init l' (add_addr l (n - 1)) then
+         n - 1
+      else
+        let aux (i:vl_index l)
+          : Lemma
+            (requires is_add l i)
+            (ensures add_payload l i = last_evict_value_or_init (prefix l i) (add_addr l i))
+            [SMTPat (is_add l i)]
+          =
+          if i = n - 1 then ()
+          else (
+            let l_i = prefix l i in
+            if not (is_add l i) then ()
+            else (
+              assert (is_add l' i  ==>
+                     add_payload l' i = last_evict_value_or_init (prefix l' i) (add_addr l' i));
+              ()
+            )
+          )
+       in
+       n
+
+(* Identify the smallest non-evict-add consistent prefix *)
+let first_non_eac_prefix (l:verifiable_log {~(evict_add_consistent l)})
+  : Tot (i:seq_index l{evict_add_consistent (prefix l i) /\
+                       (is_add l i && 
+                        add_payload l i <> last_evict_value_or_init (prefix l i)
+                                                                   (add_addr l i))}) = 
+  search_first_non_eac_prefix l
+
+(* evict add consistent is computable *)
+let is_evict_add_consistent (l:verifiable_log): 
+  Tot (b:bool{b <==> evict_add_consistent l}) = 
+  search_first_non_eac_prefix l = length l
+
+(* 
+ * for a verifiable log l, every merkle addr is associated with an ancestor identified below 
+ * - the smallest ancestor who has been added so far - as verifying ancestor. The verifying 
+ * ancestor is the one that will validate address a during Add's
+ *)
+let rec verifying_ancestor (l:verifiable_log) (a:merkle_non_root_addr): 
+  Tot (a':merkle_addr{is_proper_desc a a'}) 
+  (decreases (length l)) = 
+  let n = length l in
+  if n = 0 then (
+    lemma_root_is_univ_ancestor a;
+    merkle_root
+  )
+  else 
+    let l' = prefix l (n - 1) in
+    let va' = verifying_ancestor l' a in
+    if is_add l (n - 1) then
+      let a' = add_addr l (n - 1) in
+      if is_proper_desc a a' && is_proper_desc a' va' then a'
+      else va'
+    else va'
+
+let points_to (d:merkle_addr) (a: merkle_addr{is_proper_desc d a}) (v:sp_merkle_payload_of_addr a) : Tot bool = 
+  let dh = get_desc_hash d a v in
+  not (Empty? dh) && d = Desc?.a dh
+
+(* 
+ * If the verifying ancestor of 'a' is in the cache and address a has been added at least once, then 
+ * the ancestor payload points to a 
+ *)
+let rec lemma_verifying_ancestor_correct 
+  (l:verifiable_log) 
+  (a:merkle_non_root_addr{has_some_add l a /\ 
+                          cache_contains (cache_at_end l) (verifying_ancestor l a) /\
+                          not (points_to a (verifying_ancestor l a) (cached_payload (cache_at_end l) (verifying_ancestor l a)))})
+  : Tot hash_collision_sp (decreases (length l)) = 
+  let cache = cache_at_end l in
+  let va = verifying_ancestor l a in
+  let pva = cached_payload cache va in
+  let n = length l in 
+  (* contradiction since l has some add of a *)
+  if n = 0 then SCollision (SMkLeaf Null) (SMkLeaf Null)
+  
+  else 
+    let l' = prefix l (n - 1) in
+    let e = index l (n - 1) in
+    match e with 
+    | _ ->
+    admit()
+                                                                 
