Veritas.Merkle.fsti
@@ -127,17 +127,29 @@ val lemma_desc_transitive (a b c: bin_tree_node):
 val lemma_parent_ancestor (a: bin_tree_node{~(Root? a)}):
   Lemma (is_desc a (parent a))
 
+(* Two ancestors of a node are ancestor/descendant of one another *)
+val lemma_two_ancestors_related (d: bin_tree_node) (a1 a2: bin_tree_node):
+  Lemma (requires (is_desc d a1 /\ is_desc d a2))
+        (ensures (is_desc a1 a2 \/ is_desc a2 a1))
+
+
 (* proper descendant *)
 let is_proper_desc (d a: bin_tree_node) = is_desc d a && d <> a
 
 (* a proper descendant is a descendant of either left or right child *)
 val lemma_proper_desc_left_or_right (d: bin_tree_node) (a: bin_tree_node {is_proper_desc d a}):
-  Lemma (is_desc d (LeftChild a) /\ ~ (is_desc d (RightChild a)) /\
+  Lemma (is_desc d (LeftChild a) /\ ~ (is_desc d (RightChild a)) \/
          is_desc d (RightChild a) /\ ~ (is_desc d (LeftChild a)))
+        [SMTPat (is_proper_desc d a)]
+        
+val lemma_desc_height_monotonic (d a: bin_tree_node):
+  Lemma (requires (is_proper_desc d a))
+        (ensures (depth d > depth a))
+        [SMTPat (is_proper_desc d a)]
 
 type desc_hash = 
   | Empty: desc_hash
-  | Desc: d:merkle_addr -> h:hash_value -> desc_hash
+  | Desc: a:merkle_addr -> h:hash_value -> desc_hash
 
 type sp_merkle_payload = 
   | SMkLeaf: value:payload -> sp_merkle_payload
